src/verification/BlockVer/Bootcode.v
@@ -1,0 +1,261 @@
+From Coq Require Import
+     ZArith.ZArith
+     Lists.List
+     micromega.Lia
+     Strings.String.
+From Katamaran Require Import
+     Notations
+     Bitvector
+     Semantics.
+
+From MSP430 Require Import
+  BlockVer.Spec
+  BlockVer.Verifier
+  Machine
+  Sig.
+
+Import MSP430Program.
+Import MSP430BlockVerifExecutor.
+Import Assembly.
+
+Set Implicit Arguments.
+Import ctx.resolution.
+Import ctx.notations.
+Import bv.notations.
+Import env.notations.
+Import ListNotations.
+Import asn.notations.
+Import Erasure.notations.
+
+Module Bootcode.
+  Import Utils.
+
+  Definition asn_ipe_registers_zero {Σ} : Assertion Σ :=
+      MPUIPC0_reg    ↦ term_val ty.wordBits [bv 0]
+    ∗ MPUIPSEGB1_reg ↦ term_val ty.wordBits [bv 0]
+    ∗ MPUIPSEGB2_reg ↦ term_val ty.wordBits [bv 0].
+
+  Definition minimal_pre {Σ} : Assertion Σ :=
+      ∃ "lif", LastInstructionFetch ↦ term_var "lif"
+    ∗ ∃ "srcg1", SRCG1_reg ↦ term_var "srcg1"
+    (* ∗ asn_mpu_registers *)
+    ∗ MPUCTL0_reg ↦ term_val ty.wordBits [bv 0xA500].
+
+  Definition minimal_post {Σ} : Assertion Σ :=
+    minimal_pre.
+
+  Record BlockVerifierContract {Σ} :=
+    MkBlockVerifierContract
+      { precondition  : Assertion (Σ ▻ "a" :: ty.Address)
+      ; instrs        : list ast_with_args
+      ; postcondition : Assertion (Σ ▻ "a" :: ty.Address ▻ "an" :: ty.Address)
+      }.
+
+  Definition ValidBlockVerifierContract {Σ} (c : @BlockVerifierContract Σ) : Prop :=
+  match c with
+    {| precondition := pre; instrs := i; postcondition := post |} =>
+      safeE (* VerificationCondition *) (postprocess
+               (sblock_verification_condition
+                  (minimal_pre ∗ pre)
+                  i
+                  (minimal_post ∗ post)
+                  wnil))
+  end.
+
+  Local Notation "'{{' P '}}' i '{{' Q '}}'" :=
+    (@MkBlockVerifierContract [ctx] P%asn i Q%asn)
+      (at level 90, format "'[v' '{{'  P  '}}' '/'  i '/' '{{'  Q  '}}' ']'").
+  Local Notation "'{{' P '}}' i '{{' Q '}}' 'with' logvars" :=
+    (@MkBlockVerifierContract logvars P%asn i Q%asn)
+      (at level 90, format "'[v' '{{'  P  '}}' '/'  i '/' '{{'  Q  '}}' '/' 'with'  logvars ']'").
+
+  Local Ltac solve_bv :=
+      repeat match goal with
+        | |- context[bv.add ?x (@bv.mk ?n 0 I)] =>
+            fold (@bv.zero n)
+        | |- context[bv.add ?x bv.zero] =>
+            rewrite bv.add_zero_r
+        end.
+
+  Local Ltac symbolic_simpl :=
+    vm_compute; constructor; simpl.
+
+  Definition asn_init_pc {Σ} (pc : Term _ ty.Address) : Assertion (Σ ▻ "a" :: ty.Address) :=
+    term_var "a" = pc.
+  Definition asn_fin_pc {Σ} (pc : Term _ ty.Address) : Assertion (Σ ▻ "an" :: ty.Address) :=
+    term_var "an" = pc.
+
+  Local Notation "v -' n" :=
+    (term_binop bop.bvsub v (term_val ty.wordBits [bv n]))
+    (at level 50).
+
+  Definition asn_byte_zero {Σ} (b : Term Σ ty.byteBits) : Assertion Σ :=
+    b = term_val ty.byteBits [bv 0].
+
+  Definition saved_ptr {Σ} : Term Σ _ := term_val ty.Address [bv 0x4200].
+  Definition isp {Σ} : Term Σ _ := term_val ty.Address [bv 0x4202].
+
+  Definition byte_zero {Σ} : Term Σ _ := term_val ty.byteBits [bv 0].
+
+  Definition valid_flag {Σ} : Term Σ _ := term_val ty.wordBits [bv 0xAAAA].
+  Definition ipe_sig_valid_src {Σ} : Term Σ _ := term_val ty.Address [bv 0xFF88].
+  Definition ipe_struct_pointer_src {Σ} : Term Σ _ := term_val ty.Address [bv 0xFF8A].
+
+  Definition start_bootcode_start{Σ} : Term Σ _ := term_val ty.wordBits [bv 0].
+  Definition transfer_if_valid_struct_start {Σ} : Term Σ _ := term_val ty.wordBits [bv 0x4].
+  Definition check_struct_start {Σ} : Term Σ _ := term_val ty.wordBits [bv 0xC].
+  Definition evaluate_struct_start {Σ} : Term Σ _ := term_val ty.wordBits [bv 0x1A].
+  Definition mass_erase_start {Σ} : Term Σ _ := term_val ty.wordBits [bv 0x2E].
+  Definition end_addr {Σ} : Term Σ _ := term_val ty.wordBits [bv 0x100].
+
+  Definition asn_flag_valid {Σ} : Assertion Σ :=
+    asn_ptsto_word ipe_sig_valid_src (low valid_flag) (high valid_flag).
+
+  Definition contract_start_bootcode : BlockVerifierContract :=
+    {{
+          asn_init_pc start_bootcode_start
+        ∗ asn_ipe_registers_zero
+
+        ∗ R10_reg ↦ saved_ptr
+        ∗ (asn_ptsto_word saved_ptr byte_zero byte_zero
+           ∨ asn_ptsto_word saved_ptr (low isp) (high isp))
+    }}
+      [ tst_m R10
+      ; jnz [bv 4] (* check_struct *)]
+    {{
+          R10_reg ↦ saved_ptr
+        ∗ asn_ipe_registers_zero
+        ∗ ( asn_ptsto_word saved_ptr byte_zero byte_zero
+              ∗ asn_fin_pc transfer_if_valid_struct_start
+            ∨ asn_ptsto_word saved_ptr (low isp) (high isp)
+              ∗ asn_fin_pc check_struct_start)
+    }}.
+
+  Definition contract_transfer_if_valid_struct : BlockVerifierContract :=
+    {{
+          asn_init_pc transfer_if_valid_struct_start
+
+        ∗ asn_ipe_registers_zero
+        ∗ R10_reg ↦ saved_ptr
+        ∗ R11_reg ↦ valid_flag
+        ∗ R12_reg ↦ ipe_sig_valid_src
+        ∗ R13_reg ↦ ipe_struct_pointer_src
+
+        ∗ asn_flag_valid
+        ∗ asn_ptsto_word ipe_struct_pointer_src (low isp) (high isp)
+        ∗ asn_ptsto_word saved_ptr byte_zero byte_zero
+    }}
+      [ cmp_rm R11 R12
+      ; jnz [bv 0x34] (* TODO end *)
+      ; mov_mm R13 R10 ]
+    {{
+          asn_fin_pc check_struct_start
+
+        ∗ asn_ipe_registers_zero
+        ∗ R10_reg ↦ saved_ptr
+        ∗ R11_reg ↦ valid_flag
+        ∗ R12_reg ↦ ipe_sig_valid_src
+        ∗ R13_reg ↦ ipe_struct_pointer_src
+
+        ∗ asn_flag_valid
+        ∗ asn_ptsto_word ipe_struct_pointer_src (low isp) (high isp)
+        ∗ asn_ptsto_word saved_ptr (low isp) (high isp)
+    }}.
+
+  Definition contract_check_struct : BlockVerifierContract :=
+    {{
+          asn_init_pc check_struct_start
+
+        ∗ asn_ipe_registers_zero
+        ∗ R10_reg ↦ saved_ptr
+        ∗ R15_reg ↦ term_val ty.wordBits [bv 0xFFFF]
+        ∗ ∃ "v", R6_reg  ↦ term_var "v"
+        ∗ ∃ "v", R14_reg ↦ term_var "v"
+
+        ∗ asn_ptsto_word saved_ptr (low isp) (high isp)
+        ∗ asn_ptsto_word isp        (term_var "ipectl_l") (term_var "ipectl_h")
+        ∗ asn_ptsto_word (isp +' 2) (term_var "segb2_l") (term_var "segb2_h")
+        ∗ asn_ptsto_word (isp +' 4) (term_var "segb1_l") (term_var "segb1_h")
+        ∗ asn_ptsto_word (isp +' 6) (term_var "check_l") (term_var "check_h")
+    }}
+      [ mov_mr R10 R6
+      ; mov_rr R15 R14
+      ; xor_ar R6 R14
+      ; xor_ar R6 R14
+      ; xor_ar R6 R14
+      ; cmp_mr R6 R14
+      ; jnz [bv 0xA] (* mass_erase_init *)
+      ]
+    {{
+          ( asn_fin_pc evaluate_struct_start
+          ∨ asn_fin_pc mass_erase_start)
+
+        ∗ asn_ipe_registers_zero
+        ∗ R10_reg ↦ saved_ptr
+        ∗ R15_reg ↦ term_val ty.wordBits [bv 0xFFFF]
+        ∗ R6_reg ↦ isp +' 6
+        ∗ ∃ "v", R14_reg ↦ term_var "v"
+
+        ∗ asn_ptsto_word saved_ptr  (low isp) (high isp)
+        ∗ asn_ptsto_word isp        (term_var "ipectl_l") (term_var "ipectl_h")
+        ∗ asn_ptsto_word (isp +' 2) (term_var "segb2_l") (term_var "segb2_h")
+        ∗ asn_ptsto_word (isp +' 4) (term_var "segb1_l") (term_var "segb1_h")
+        ∗ asn_ptsto_word (isp +' 6) (term_var "check_l") (term_var "check_h")
+
+    }} with [ "ipectl_l" :: ty.byteBits; "ipectl_h" :: ty.byteBits
+            ; "segb2_l"  :: ty.byteBits; "segb2_h"  :: ty.byteBits
+            ; "segb1_l"  :: ty.byteBits; "segb1_h"  :: ty.byteBits
+            ; "check_l"  :: ty.byteBits; "check_h"  :: ty.byteBits ].
+
+  Definition contract_evaluate_struct : BlockVerifierContract :=
+    {{
+         asn_init_pc evaluate_struct_start
+
+       ∗ asn_ipe_registers_zero
+       ∗ R6_reg ↦ isp +' 6
+       ∗ R7_reg ↦ MPUIPC0_addr
+       ∗ R8_reg ↦ MPUIPSEGB2_addr
+       ∗ R9_reg ↦ MPUIPSEGB1_addr
+
+       ∗ asn_ptsto_word (isp +' 4) (low (term_var "segb1")) (high (term_var "segb1"))
+       ∗ asn_ptsto_word (isp +' 2) (low (term_var "segb2")) (high (term_var "segb2"))
+       ∗ asn_ptsto_word isp (low (term_var "ipectl")) (high (term_var "ipectl"))
+    }}
+      [ mov_im R6 (bv.of_Z (-2)%Z) R9
+      ; mov_im R6 (bv.of_Z (-4)%Z) R8
+      ; mov_im R6 (bv.of_Z (-6)%Z) R7
+      ; jump JMP [bv 105] (* end *) ]
+    {{
+         asn_fin_pc end_addr
+
+       ∗ MPUIPC0_reg    ↦ term_var "ipectl"
+       ∗ MPUIPSEGB1_reg ↦ term_var "segb1"
+       ∗ MPUIPSEGB2_reg ↦ term_var "segb2"
+
+       ∗ R6_reg ↦ isp +' 6
+       ∗ R7_reg ↦ MPUIPC0_addr
+       ∗ R8_reg ↦ MPUIPSEGB2_addr
+       ∗ R9_reg ↦ MPUIPSEGB1_addr
+
+       ∗ asn_ptsto_word (isp +' 4) (low (term_var "segb1")) (high (term_var "segb1"))
+       ∗ asn_ptsto_word (isp +' 2) (low (term_var "segb2")) (high (term_var "segb2"))
+       ∗ asn_ptsto_word isp (low (term_var "ipectl")) (high (term_var "ipectl"))
+    }} with [ "ipectl" :: ty.wordBits; "segb1" :: ty.wordBits; "segb2" :: ty.wordBits ].
+
+  Lemma valid_start_bootcode : ValidBlockVerifierContract contract_start_bootcode.
+  Proof. now symbolic_simpl. Qed.
+
+  Lemma valid_transfer_if_valid_struct : ValidBlockVerifierContract contract_transfer_if_valid_struct.
+  Proof. now symbolic_simpl. Qed.
+
+  Lemma valid_check_struct : ValidBlockVerifierContract contract_check_struct.
+  Proof. now symbolic_simpl. Qed.
+
+  Lemma valid_evaluate_struct : ValidBlockVerifierContract contract_evaluate_struct.
+  Proof.
+    symbolic_simpl.
+    intuition;
+      unfold bv.app; unfold bv.take; unfold bv.drop;
+      destruct bv.appView; reflexivity.
+  Qed.
+End Bootcode.
